Coq/Simplicity/Primitive.v
@@ -1,0 +1,121 @@
+Require Import Util.List.
+Require Import Strings.String.
+Require Import Util.PackedClass.
+Require Import Util.Monad.
+Require Import Util.Monad.Reader.
+Require Import Util.Option.
+
+Require Import Simplicity.Alg.
+Require Import Simplicity.MerkleRoot.
+Require Import Simplicity.Ty.
+
+Set Implicit Arguments.
+Import ListNotations.
+
+Definition primitivePrefix primName := (MerkleRoot.prefix ++ ["Primitive"%string; primName])%list.
+
+Module Type PrimitiveSig.
+
+Parameter t : Ty -> Ty -> Set.
+Parameter tag : forall {A B}, t A B -> hash256.
+
+Parameter env : Set.
+Parameter sem : env -> forall {A B}, t A B -> A -> option B.
+
+End PrimitiveSig.
+
+Module Primitive (Prim : PrimitiveSig).
+
+Record mixin (term : Ty -> Ty -> Type) := Mixin
+{ prim : forall {A B}, Prim.t A B -> term A B
+}.
+
+Record class (term : Ty -> Ty -> Type) := Class
+{ base :> Assertion.class term
+; ext  :> mixin term
+}.
+
+Structure Algebra := _Pack { domain :> Ty -> Ty -> Type; class_of : class domain }.
+
+Definition packager dom (p0 : mixin dom) :=
+ [find a  | Assertion.domain a ~ dom | "is not a Assertion algebra" ]
+ [find ac | Assertion.class_of a ~ ac ]
+ [find p  | p ~ p0 | "is not the right mixin" ]
+ @_Pack dom (@Class dom ac p).
+
+Notation Pack dom p := (@packager dom p _ id _ id _ id).
+
+Canonical Structure toCore (alg : Algebra) : Core.Algebra :=
+  Core.Pack alg (class_of alg).
+Canonical Structure toAssertion (alg : Algebra) : Assertion.Algebra :=
+  Assertion.Pack alg (class_of alg).
+
+Module Combinators.
+
+Definition prim {A B} {alg : Algebra} : Prim.t A B -> alg A B := prim (class_of alg).
+
+End Combinators.
+
+Module Parametric.
+Import Combinators.
+
+Record mixin {alg1 alg2 : Algebra} (rel : forall {A B}, alg1 A B -> alg2 A B -> Prop) :=
+ { _ : forall A B (p : Prim.t A B), rel (prim p) (prim p)
+ }.
+
+Record class {alg1 alg2 : Algebra} (rel : forall {A B}, alg1 A B -> alg2 A B -> Prop) :=
+ { base :> Assertion.Parametric.class (@rel)
+ ; ext :> mixin (@rel)
+ }.
+
+Record Rel (alg1 alg2 : Algebra) := Pack
+ { rel :> forall {A B}, alg1 A B -> alg2 A B -> Prop
+ ; class_of : class (@rel)
+ }.
+
+End Parametric.
+
+Section Reynolds.
+Local Coercion Parametric.rel : Parametric.Rel >-> Funclass.
+
+Definition Reynolds {A B} (x y : forall (alg : Algebra), alg A B) : Prop :=
+  forall alg1 alg2 (R : Parametric.Rel alg1 alg2), R A B (x alg1) (y alg2).
+
+Definition Parametric {A B} (x : forall (alg : Algebra), alg A B) : Prop := Reynolds x x.
+End Reynolds.
+
+Module Theory.
+Export Combinators.
+Coercion Parametric.rel : Parametric.Rel >-> Funclass.
+
+Lemma prim_Parametric {alg1 alg2 : Algebra} (R : Parametric.Rel alg1 alg2)
+  {A B} (p : Prim.t A B) : R A B (prim p) (prim p).
+Proof.
+destruct R as [R [Rb []]].
+cbn; auto.
+Qed.
+Hint Immediate prim_Parametric : parametricity.
+
+Definition primSem M A B := Kleisli (ReaderT Prim.env M) A B.
+
+Definition PrimSem_mixin (M : CIMonadZero) : Primitive.mixin (primSem M) :=
+  {| Primitive.prim A B p := fun a e => optionZero (Prim.sem e p a)
+   |}.
+
+Canonical Structure CorePrimSem (M : CIMonad) : Core.Algebra :=
+  Core.Pack (primSem M) (CoreSem_mixin (ReaderT_CIMonad Prim.env M)).
+Canonical Structure AssertionPrimSem (M : CIMonadZero) : Assertion.Algebra :=
+  Assertion.Pack (primSem M) (AssertionSem_mixin (ReaderT_CIMonadZero Prim.env M)).
+Canonical Structure AssertionSem (M : CIMonadZero) : Primitive.Algebra :=
+  Primitive.Pack (primSem M) (PrimSem_mixin M).
+
+Definition CommitmentRoot_Primitive_mixin : Primitive.mixin CommitmentRoot :=
+ {| Primitive.prim A B p := Prim.tag p
+  |}.
+
+Canonical Structure CommitmentRoot_Primitive_alg : Primitive.Algebra :=
+  Primitive.Pack CommitmentRoot CommitmentRoot_Primitive_mixin.
+
+End Theory.
+
+End Primitive.
