Coq/Simplicity/Primitive/Bitcoin.v
@@ -1,0 +1,219 @@
+Require Import ZArith.
+Require Import String.
+Require Import Util.List.
+Require Import compcert.lib.Integers.
+Global Unset Asymmetric Patterns. (* the VST library does a Global Set so we must unset it. *)
+
+Require Import Simplicity.Digest.
+Require Simplicity.MerkleRoot.
+Require Import Simplicity.Primitive.
+Require Import Simplicity.Ty.
+Require Import Simplicity.SHA256.
+Require Import Simplicity.Word.
+
+Set Primitive Projections.
+Set Implicit Arguments.
+
+Import ListNotations.
+
+Section DataTypes.
+
+Definition MAX_MONEY : Z := 21000000 * 10^8.
+Notation moneyRange x := (-1 < x < Z.succ MAX_MONEY)%Z.
+
+Definition lock := int.
+Definition script := list byte.
+
+Record outpoint : Set :=
+ { opHash : hash256
+ ; opIndex : int
+ }.
+
+Record sigTxInput : Set :=
+ { sigTxiPreviousOutpoint : outpoint
+ ; sigTxiValue : int64
+ ; sigTxiSequence : int
+ ; sigTxiValue_bound : moneyRange (Int64.signed sigTxiValue)
+ }.
+
+Record txOutput : Set :=
+ { txoValue : int64
+ ; txoScript : script
+ ; txoValue_bound : moneyRange (Int64.signed txoValue)
+ ; txoScript_bound : (Zlength txoScript < Int.modulus)%Z
+ }.
+
+Record sigTx : Set :=
+ { sigTxVersion : int
+ ; sigTxIn : list sigTxInput
+ ; sigTxOut : list txOutput
+ ; sigTxLock : lock
+ ; sigTxInBounds : (0 < Zlength sigTxIn < Z.succ Int64.modulus)%Z
+ ; sigTxOutBounds : (0 < Zlength sigTxOut < Z.succ Int.modulus)%Z
+ ; sigTxTotalInValue : Z := Z_sum (map (fun i => Int64.signed (sigTxiValue i)) sigTxIn)
+ ; sigTxTotalOutValue : Z := Z_sum (map (fun i => Int64.signed (txoValue i)) sigTxOut)
+ ; sigTxFee : Z := sigTxTotalOutValue - sigTxTotalInValue
+ ; sigTxTotalInValue_bound : moneyRange sigTxTotalInValue
+ ; sigTxTotalOutValue_bound : moneyRange sigTxTotalOutValue
+ ; sigTxFee_bound : moneyRange sigTxFee
+ }.
+
+End DataTypes.
+
+Section Serialization.
+
+Definition putHash256le (x : hash256) : list byte :=
+  map Byte.repr (hash256_to_Zlist x).
+
+Definition putInt64le (x : Int64.int) : list byte :=
+let z := Int64.unsigned x in
+map (fun i => Byte.repr (z / two_power_nat (i*Byte.wordsize))%Z) (seq 0 8).
+
+Definition putInt32le (x : Int.int) : list byte :=
+let z := Int.unsigned x in
+map (fun i => Byte.repr (z / two_power_nat (i*Byte.wordsize))%Z) (seq 0 4).
+
+Definition putVarInt (x : Int64.int) : list byte :=
+let z := Int64.unsigned x in
+  if (Z_lt_le_dec z 253)
+  then [ Byte.repr z ]
+  else if (Z_lt_le_dec z (two_power_nat 16))
+  then Byte.repr 253 :: map (fun i => Byte.repr (z / two_power_nat (i*Byte.wordsize))%Z) (seq 0 2)
+  else if (Z_lt_le_dec z Int.modulus)
+  then Byte.repr 254 :: putInt32le (Int.repr z)
+  else Byte.repr 255 :: putInt64le (Int64.repr z).
+
+Definition putScript (x : script) : list byte :=
+let z := Int64.repr (Zlength x) in
+    putVarInt z ++ x.
+
+Definition putOutpoint (x : outpoint) : list byte :=
+    putHash256le (opHash x)
+ ++ putInt32le (opIndex x).
+
+Definition putTxOutput (x : txOutput) : list byte :=
+    putInt64le (txoValue x)
+ ++ putScript (txoScript x).
+
+End Serialization.
+
+Module Bitcoin <: PrimitiveSig.
+
+Inductive prim : Ty -> Ty -> Set :=
+| Version : prim Unit Word32
+| LockTime : prim Unit Word32
+| InputsHash : prim Unit Word256
+| OutputsHash : prim Unit Word256
+| MaxInput : prim Unit Word64
+| TotalInputValue : prim Unit Word64
+| CurrentPrevOutpoint : prim Unit (Prod Word256 Word32)
+| CurrentValue : prim Unit Word64
+| CurrentSequence : prim Unit Word32
+| CurrentIndex : prim Unit Word64
+| InputPrevOutpoint : prim Word64 (Sum Unit (Prod Word256 Word32))
+| InputValue : prim Word64 (Sum Unit Word64)
+| InputSequence : prim Word64 (Sum Unit Word32)
+| MaxOutput : prim Unit Word32
+| TotalOutputValue : prim Unit Word64
+| OutputValue : prim Word32 (Sum Unit Word64)
+| OutputScriptHash : prim Word32 (Sum Unit Word256)
+| ScirptCMR : prim Unit Word256.
+Definition t := prim.
+
+Definition primName : string := "Bitcoin".
+
+Definition name {a b} (p : t a b) : string :=
+match p with
+| Version => "version"
+| LockTime => "locktime"
+| InputsHash => "inputsHash"
+| OutputsHash => "outputsHash"
+| MaxInput => "maxInput"
+| TotalInputValue => "totalInputValue"
+| CurrentPrevOutpoint => "currentPrevOutpoint"
+| CurrentValue => "currentValue"
+| CurrentSequence => "currentSequence"
+| CurrentIndex => "currentIndex"
+| InputPrevOutpoint => "inputPrevOutpoint"
+| InputValue => "inputValue"
+| InputSequence => "inputSequence"
+| MaxOutput => "maxOutput"
+| TotalOutputValue => "totalOutputValue"
+| OutputValue => "outputValue"
+| OutputScriptHash => "outputScriptHash"
+| ScriptCMR => "scriptCMR"
+end.
+
+Section Tag.
+
+Let tag_def {A B} (p : t A B) : hash256.
+pose (nm := name p).
+revert p nm; intros [] nm;
+exact (MerkleRoot.tag (primitivePrefix primName ++ [nm]) refl_equal).
+Defined.
+
+(* Using Eval vm_compute lets us precompute all the tags for all our primitives *)
+Definition tag {A B} (p : t A B) := Eval vm_compute in (tag_def p).
+(* Try running *)
+(* Print tag.  *)
+
+End Tag.
+
+Record enviroment :=
+{ envTx : sigTx
+; envIx : nat
+; envScriptCMR : hash256
+; envIxBounded : envIx < length (sigTxIn envTx)
+}.
+Definition env := enviroment.
+
+Section primSem.
+
+Let cast {A : Ty} (x : option A) : tySem (Unit + A) :=
+match x with
+| Some a => inr a
+| None => inl tt
+end.
+
+Let encodeOutpoint (op : outpoint) : tySem (Word256 * Word32) :=
+ (repr_Hash_inv (opHash op), fromZ (Int.unsigned (opIndex op)) : Word32).
+
+Definition sem (e : env) {A B} (p : t A B) : A -> option B :=
+let tx := envTx e in
+let ix := envIx e in
+let currentInput {A : Ty} (f : sigTxInput -> A) := option_map f (nth_error (sigTxIn tx) ix) in
+let atInput {A : Ty} (f : sigTxInput -> A) (i : Word64) :=
+  Some (cast (option_map f (nth_error (sigTxIn tx) (Z.to_nat (toZ i))))) in
+let atOutput {A : Ty} (f : txOutput -> A) (i : Word32) :=
+  Some (cast (option_map f (nth_error (sigTxOut tx) (Z.to_nat (toZ i))))) in
+let outputsHash := byteStringHash (concat (map putTxOutput (sigTxOut tx))) in
+let inputsHash :=
+  let go i := putOutpoint (sigTxiPreviousOutpoint i) ++ putInt32le (sigTxiSequence i) in
+  byteStringHash (concat (map go (sigTxIn tx))) in
+match p with
+| Version => fun _ => Some (fromZ (Int.signed (sigTxVersion tx)))
+| LockTime => fun _ => Some (fromZ (Int.unsigned (sigTxLock tx)))
+| InputsHash => fun _ => Some (repr_Hash_inv inputsHash)
+| OutputsHash => fun _ => Some (repr_Hash_inv outputsHash)
+| MaxInput => fun _ => Some (fromZ (Zpred (Zlength (sigTxIn tx))))
+| TotalInputValue => fun _ => Some (fromZ (sigTxTotalInValue tx))
+| CurrentPrevOutpoint => fun _ => currentInput (fun txi => encodeOutpoint (sigTxiPreviousOutpoint txi))
+| CurrentValue => fun _ => currentInput (fun txi => fromZ (Int64.signed (sigTxiValue txi)))
+| CurrentSequence => fun _ => currentInput (fun txi => fromZ (Int.unsigned (sigTxiSequence txi)))
+| CurrentIndex => fun _ => Some (fromZ (Z.of_nat ix))
+| InputPrevOutpoint => atInput (fun txi => encodeOutpoint (sigTxiPreviousOutpoint txi))
+| InputValue => atInput (fun txi => fromZ (Int64.signed (sigTxiValue txi)))
+| InputSequence => atInput (fun txi => fromZ (Int.unsigned (sigTxiSequence txi)))
+| MaxOutput => fun _ => Some (fromZ (Zpred (Zlength (sigTxOut tx))))
+| TotalOutputValue => fun _ => Some (fromZ (sigTxTotalOutValue tx))
+| OutputValue => atOutput (fun txout => fromZ (Int64.signed (txoValue txout)))
+| OutputScriptHash => atOutput (fun txout => repr_Hash_inv (byteStringHash (txoScript txout)))
+| ScriptCMR => fun _ => Some (repr_Hash_inv (envScriptCMR e))
+end.
+
+End primSem.
+
+End Bitcoin.
+
+Module PrimitiveBitcoin := Primitive Bitcoin.
+Export PrimitiveBitcoin.Theory.
