Simplicity.Coq.nix
@@ -2,9 +2,10 @@
 stdenv.mkDerivation {
   name = "Simplicity-coq-0.0.0";
   src = lib.sourceFilesBySuffices
-      (lib.sourceByRegex ./Coq ["Simplicity" "Util" ".*v$"])
+      (lib.sourceByRegex ./Coq ["Simplicity" "Simplicity/.*" "Util" "Util/.*"])
     [".v"];
   postConfigure = ''
+    shopt -s globstar
     coq_makefile -Q Simplicity Simplicity -Q Util Util **/*.v > Makefile
   '';
   buildInputs = [ coq ];
